Add UpperBound_A.v && strengthen CsemC

cfrontend/CsemC.v
@@ -15,6 +15,12 @@ Set Implicit Arguments.
 
 
 
+Definition is_call_cont_strong (k0: cont): Prop :=
+  match k0 with
+  | Kcall _ _ _ _ _ => True
+  | _ => False
+  end
+.
 
 Section CEXTRA.
 
@@ -89,17 +95,18 @@ Section MODSEM.
 
   Inductive at_external : state -> Args.t -> Prop :=
   | at_external_intro
-      fptr_arg tyf vs_arg sg_arg targs tres cconv k m0
+      fptr_arg tyf vs_arg sg_arg targs tres cconv k0 m0
       (EXTERNAL: ge.(Genv.find_funct) fptr_arg = None)
       (SIG: exists skd, skenv_link.(Genv.find_funct) fptr_arg = Some skd
                    /\ (SkEnv.get_sig skd = sg_arg
                       -> tyf = Tfunction targs tres cconv
                       -> signature_of_type targs tres cconv = sg_arg))
                    (* /\ type_of_fundef skd = tyf) *)
+      (CALL: is_call_cont_strong k0)
     (* how can i check sg_args and tyf are same type? *)
     (* typ_of_type function is a projection type to typ. it delete some info *)
     :
-      at_external (Callstate fptr_arg tyf vs_arg k m0)
+      at_external (Callstate fptr_arg tyf vs_arg k0 m0)
                   (Args.mk fptr_arg vs_arg m0)
   .
 
